cleaning WordInterval

thy/IP_Addresses/WordInterval.thy
@@ -26,25 +26,28 @@ subsection\<open>Semantics\<close>
 
 subsection\<open>Basic operations\<close>
   fun wordinterval_element :: "'a::len0 word \<Rightarrow> 'a::len0 wordinterval \<Rightarrow> bool" where
-    "wordinterval_element el (WordInterval s e) = (s \<le> el \<and> el \<le> e)" |
-    "wordinterval_element el (RangeUnion r1 r2) = (wordinterval_element el r1 \<or> wordinterval_element el r2)"
-  lemma wordinterval_element_set_eq[simp]: "wordinterval_element el rg = (el \<in> wordinterval_to_set rg)"
+    "wordinterval_element el (WordInterval s e) \<longleftrightarrow> s \<le> el \<and> el \<le> e" |
+    "wordinterval_element el (RangeUnion r1 r2) \<longleftrightarrow>
+                                            wordinterval_element el r1 \<or> wordinterval_element el r2"
+  lemma wordinterval_element_set_eq[simp]:
+    "wordinterval_element el rg = (el \<in> wordinterval_to_set rg)"
     by(induction rg rule: wordinterval_element.induct) simp_all
   
-  definition wordinterval_union :: "'a::len0 wordinterval \<Rightarrow> 'a::len0 wordinterval \<Rightarrow> 'a::len0 wordinterval" where 
+  definition wordinterval_union
+    :: "'a::len0 wordinterval \<Rightarrow> 'a::len0 wordinterval \<Rightarrow> 'a::len0 wordinterval" where 
     "wordinterval_union r1 r2 = RangeUnion r1 r2"
-  lemma wordinterval_union_set_eq[simp]: "wordinterval_to_set (wordinterval_union r1 r2) = wordinterval_to_set r1 \<union> wordinterval_to_set r2"
+  lemma wordinterval_union_set_eq[simp]:
+    "wordinterval_to_set (wordinterval_union r1 r2) = wordinterval_to_set r1 \<union> wordinterval_to_set r2"
     unfolding wordinterval_union_def by simp
   
   fun wordinterval_empty :: "'a::len0 wordinterval \<Rightarrow> bool" where
-    "wordinterval_empty (WordInterval s e) = (e < s)" |
-    "wordinterval_empty (RangeUnion r1 r2) = (wordinterval_empty r1 \<and> wordinterval_empty r2)"
+    "wordinterval_empty (WordInterval s e) \<longleftrightarrow> e < s" |
+    "wordinterval_empty (RangeUnion r1 r2) \<longleftrightarrow> wordinterval_empty r1 \<and> wordinterval_empty r2"
   lemma wordinterval_empty_set_eq[simp]: "wordinterval_empty r \<longleftrightarrow> wordinterval_to_set r = {}"
     by(induction r) auto
   
-
-  (*len, not len0*)
-  definition Empty_WordInterval :: "'a::len wordinterval" where "Empty_WordInterval \<equiv> WordInterval 1 0"
+  definition Empty_WordInterval :: "'a::len wordinterval" where
+    "Empty_WordInterval \<equiv> WordInterval 1 0"
   lemma wordinterval_empty_Empty_WordInterval: "wordinterval_empty Empty_WordInterval"
     by(simp add: Empty_WordInterval_def)
   lemma Empty_WordInterval_set_eq[simp]: "wordinterval_to_set Empty_WordInterval = {}"
@@ -67,7 +70,8 @@ subsection\<open>WordInterval and Lists\<close>
     "l2wi ((s,e)#rs) = (RangeUnion (WordInterval s e) (l2wi rs))"
   
 
-  lemma l2wi_append: "wordinterval_to_set (l2wi (l1@l2)) = wordinterval_to_set (l2wi l1) \<union> wordinterval_to_set (l2wi l2)"
+  lemma l2wi_append: "wordinterval_to_set (l2wi (l1@l2)) =
+                      wordinterval_to_set (l2wi l1) \<union> wordinterval_to_set (l2wi l2)"
     proof(induction l1 arbitrary: l2 rule:l2wi.induct)
     case 1 thus ?case by simp
     next
@@ -90,32 +94,58 @@ subsection\<open>WordInterval and Lists\<close>
 
 
 
-subsection\<open>Optimizing and minimizing @{typ "('a::len0) wordinterval"}s\<close>
+subsection\<open>Optimizing and minimizing @{typ "('a::len) wordinterval"}s\<close>
 text\<open>Removing empty intervals\<close>
 context
 begin
-  fun wordinterval_optimize_empty where
-    "wordinterval_optimize_empty (RangeUnion r1 r2) = (let r1o = wordinterval_optimize_empty r1 in (let r2o = wordinterval_optimize_empty r2 in (
-      if wordinterval_empty r1o then r2o else (if wordinterval_empty r2o then r1o else (RangeUnion r1o r2o)))))" |
+  fun wordinterval_optimize_empty :: "'a::len0 wordinterval \<Rightarrow> 'a wordinterval" where
+    "wordinterval_optimize_empty (RangeUnion r1 r2) = (let r1o = wordinterval_optimize_empty r1;
+                                                           r2o = wordinterval_optimize_empty r2
+      in if
+        wordinterval_empty r1o
+      then
+        r2o
+      else if
+        wordinterval_empty r2o
+      then
+        r1o
+      else
+        RangeUnion r1o r2o)" |
     "wordinterval_optimize_empty r = r"
-  lemma wordinterval_optimize_empty_set_eq[simp]: "wordinterval_to_set (wordinterval_optimize_empty r) = wordinterval_to_set r"
+  lemma wordinterval_optimize_empty_set_eq[simp]:
+    "wordinterval_to_set (wordinterval_optimize_empty r) = wordinterval_to_set r"
     by(induction r) (simp_all add: Let_def)
 
-  lemma wordinterval_optimize_empty_double: "wordinterval_optimize_empty (wordinterval_optimize_empty r) = wordinterval_optimize_empty r"
+  lemma wordinterval_optimize_empty_double:
+    "wordinterval_optimize_empty (wordinterval_optimize_empty r) = wordinterval_optimize_empty r"
     by(induction r) (simp_all add: Let_def)
 
-  private fun wordinterval_empty_shallow where
-    "wordinterval_empty_shallow (WordInterval s e) = (e < s)" |
-    "wordinterval_empty_shallow (RangeUnion _ _) = False"
-  private lemma helper_optimize_shallow: "wordinterval_empty_shallow (wordinterval_optimize_empty r) = wordinterval_empty (wordinterval_optimize_empty r)"
+  private fun wordinterval_empty_shallow :: "'a::len0 wordinterval \<Rightarrow> bool"  where
+    "wordinterval_empty_shallow (WordInterval s e) \<longleftrightarrow> e < s" |
+    "wordinterval_empty_shallow (RangeUnion _ _) \<longleftrightarrow> False"
+  private lemma helper_optimize_shallow:
+    "wordinterval_empty_shallow (wordinterval_optimize_empty r) =
+      wordinterval_empty (wordinterval_optimize_empty r)"
     by(induction r) fastforce+
   private fun wordinterval_optimize_empty2 where
-    "wordinterval_optimize_empty2 (RangeUnion r1 r2) = (let r1o = wordinterval_optimize_empty r1 in (let r2o = wordinterval_optimize_empty r2 in (
-      if wordinterval_empty_shallow r1o then r2o else (if wordinterval_empty_shallow r2o then r1o else (RangeUnion r1o r2o)))))" |
+    "wordinterval_optimize_empty2 (RangeUnion r1 r2) = (let r1o = wordinterval_optimize_empty r1;
+                                                            r2o = wordinterval_optimize_empty r2
+      in if
+        wordinterval_empty_shallow r1o
+      then
+        r2o
+      else if
+        wordinterval_empty_shallow r2o
+      then
+        r1o
+      else
+        RangeUnion r1o r2o)" |
     "wordinterval_optimize_empty2 r = r"
-  lemma wordinterval_optimize_empty_code[code_unfold]: "wordinterval_optimize_empty = wordinterval_optimize_empty2"
+  lemma wordinterval_optimize_empty_code[code_unfold]:
+    "wordinterval_optimize_empty = wordinterval_optimize_empty2"
     by (subst fun_eq_iff, clarify, rename_tac r, induct_tac r)
-       (unfold wordinterval_optimize_empty.simps wordinterval_optimize_empty2.simps Let_def helper_optimize_shallow, simp_all)
+       (unfold wordinterval_optimize_empty.simps wordinterval_optimize_empty2.simps
+               Let_def helper_optimize_shallow, simp_all)
 end
 
 
@@ -131,31 +161,42 @@ begin
     "interval_of (s,e) = {s .. e}"
   declare interval_of.simps[simp del]
 
-  private definition disjoint_intervals :: "(('a::len0) word \<times> ('a::len0) word) \<Rightarrow> ('a word \<times> 'a word) \<Rightarrow> bool" where
+  private definition disjoint_intervals
+    :: "(('a::len0) word \<times> ('a::len0) word) \<Rightarrow> ('a word \<times> 'a word) \<Rightarrow> bool"
+  where
     "disjoint_intervals A B \<equiv> disjoint (interval_of A) (interval_of B)"
 
-  private definition not_disjoint_intervals :: "(('a::len0) word \<times> ('a::len0) word) \<Rightarrow> ('a word \<times> 'a word) \<Rightarrow> bool" where
+  private definition not_disjoint_intervals
+    :: "(('a::len0) word \<times> ('a::len0) word) \<Rightarrow> ('a word \<times> 'a word) \<Rightarrow> bool"
+  where
     "not_disjoint_intervals A B \<equiv> \<not> disjoint (interval_of A) (interval_of B)"
 
-  private lemma [code]: "not_disjoint_intervals A B = (case A of (s,e) \<Rightarrow> case B of (s',e') \<Rightarrow> s \<le> e' \<and> s' \<le> e \<and> s \<le> e \<and> s' \<le> e')"
+  private lemma [code]:
+    "not_disjoint_intervals A B =
+      (case A of (s,e) \<Rightarrow> case B of (s',e') \<Rightarrow> s \<le> e' \<and> s' \<le> e \<and> s \<le> e \<and> s' \<le> e')"
     apply(cases A, cases B)
     apply(simp add: not_disjoint_intervals_def interval_of.simps disjoint_def)
     done
 
-  private lemma [code]: "disjoint_intervals A B = (case A of (s,e) \<Rightarrow> case B of (s',e') \<Rightarrow> s > e' \<or> s' > e \<or> s > e \<or> s' > e')"
+  private lemma [code]:
+    "disjoint_intervals A B =
+      (case A of (s,e) \<Rightarrow> case B of (s',e') \<Rightarrow> s > e' \<or> s' > e \<or> s > e \<or> s' > e')"
     apply(cases A, cases B)
     apply(simp add: disjoint_intervals_def interval_of.simps disjoint_def)
     by fastforce
 
 
   text\<open>BEGIN merging overlapping intervals\<close>
-  (*result has no empty intervals and all are disjoiint. merging things such as [1,7] [8,10] would still be possible*)
-  private fun merge_overlap :: "(('a::len0) word \<times> ('a::len0) word) \<Rightarrow> ('a word \<times> 'a word) list \<Rightarrow> ('a word \<times> 'a word) list" where
-   "merge_overlap s [] = [s]" |
-   "merge_overlap (s,e) ((s',e')#ss) = (
-      if not_disjoint_intervals (s,e) (s',e')
-      then (min s s', max e e')#ss
-      else (s',e')#merge_overlap (s,e) ss)"
+  (*result has no empty intervals and all are disjoint.
+    merging things such as [1,7] [8,10] would still be possible*)
+  private fun merge_overlap
+    :: "(('a::len0) word \<times> ('a::len0) word) \<Rightarrow> ('a word \<times> 'a word) list \<Rightarrow> ('a word \<times> 'a word) list"
+  where
+    "merge_overlap s [] = [s]" |
+    "merge_overlap (s,e) ((s',e')#ss) = (
+       if not_disjoint_intervals (s,e) (s',e')
+       then (min s s', max e e')#ss
+       else (s',e')#merge_overlap (s,e) ss)"
 
   private lemma not_disjoint_union:
       fixes s :: "('a::len0) word"
@@ -169,7 +210,7 @@ begin
   private lemma merge_overlap_helper1: "interval_of A \<subseteq> (\<Union>s \<in> set ss. interval_of s) \<Longrightarrow>
       (\<Union>s \<in> set (merge_overlap A ss). interval_of s) = (\<Union>s \<in> set ss. interval_of s)"
     apply(induction ss)
-     apply(simp)
+     apply(simp; fail)
     apply(rename_tac x xs)
     apply(cases A, rename_tac a b)
     apply(case_tac x)
@@ -184,7 +225,7 @@ begin
   private lemma merge_overlap_helper2: "\<exists>s'\<in>set ss. \<not> disjoint (interval_of A) (interval_of s') \<Longrightarrow>
           interval_of A \<union> (\<Union>s \<in> set ss. interval_of s) = (\<Union>s \<in> set (merge_overlap A ss). interval_of s)"
     apply(induction ss)
-     apply(simp)
+     apply(simp; fail)
     apply(rename_tac x xs)
     apply(cases A, rename_tac a b)
     apply(case_tac x)
@@ -195,7 +236,9 @@ begin
     apply(simp)
     by blast
 
-  private lemma merge_overlap_length: "\<exists>s' \<in> set ss. \<not> disjoint (interval_of A) (interval_of s') \<Longrightarrow> length (merge_overlap A ss) = length ss"
+  private lemma merge_overlap_length:
+    "\<exists>s' \<in> set ss. \<not> disjoint (interval_of A) (interval_of s') \<Longrightarrow>
+      length (merge_overlap A ss) = length ss"
     apply(induction ss)
      apply(simp)
     apply(rename_tac x xs)
@@ -204,9 +247,12 @@ begin
     apply(simp add: not_disjoint_intervals_def interval_of.simps)
     done
 
-  value[code] "merge_overlap (1:: 16 word,2)"
+  lemma "merge_overlap (1:: 16 word,2) [(1, 7)] = [(1, 7)]" by eval
+  lemma "merge_overlap (1:: 16 word,2) [(2, 7)] = [(1, 7)]" by eval
+  lemma "merge_overlap (1:: 16 word,2) [(3, 7)] = [(3, 7), (1,2)]" by eval
 
-  private function listwordinterval_compress :: "(('a::len0) word \<times> ('a::len0) word) list \<Rightarrow> ('a word \<times> 'a word) list" where
+  private function listwordinterval_compress
+    :: "(('a::len0) word \<times> ('a::len0) word) list \<Rightarrow> ('a word \<times> 'a word) list" where
     "listwordinterval_compress [] = []" |
     "listwordinterval_compress (s#ss) = (
             if \<forall>s' \<in> set ss. disjoint_intervals s s'
@@ -220,7 +266,8 @@ begin
    apply(simp)
   using disjoint_intervals_def merge_overlap_length by fastforce
 
-  private lemma listwordinterval_compress: "(\<Union>s \<in> set (listwordinterval_compress ss). interval_of s) = (\<Union>s \<in> set ss. interval_of s)"
+  private lemma listwordinterval_compress:
+    "(\<Union>s \<in> set (listwordinterval_compress ss). interval_of s) = (\<Union>s \<in> set ss. interval_of s)"
     apply(induction ss rule: listwordinterval_compress.induct)
      apply(simp)
     apply(simp)
@@ -230,13 +277,16 @@ begin
     apply(simp)
     done
 
-  value[code] "listwordinterval_compress [(1::32 word,3), (8,10), (2,5), (3,7)]"
+  lemma "listwordinterval_compress [(1::32 word,3), (8,10), (2,5), (3,7)] = [(8, 10), (1, 7)]"
+    by eval
 
-  private lemma A_in_listwordinterval_compress: "A \<in> set (listwordinterval_compress ss) \<Longrightarrow> interval_of A \<subseteq> (\<Union>s \<in> set ss. interval_of s)"
+  private lemma A_in_listwordinterval_compress: "A \<in> set (listwordinterval_compress ss) \<Longrightarrow>
+    interval_of A \<subseteq> (\<Union>s \<in> set ss. interval_of s)"
     using listwordinterval_compress by blast
 
   private lemma listwordinterval_compress_disjoint: 
-    "A \<in> set (listwordinterval_compress ss) \<Longrightarrow> B \<in> set (listwordinterval_compress ss) \<Longrightarrow> A \<noteq> B \<Longrightarrow> disjoint (interval_of A) (interval_of B)"
+    "A \<in> set (listwordinterval_compress ss) \<Longrightarrow> B \<in> set (listwordinterval_compress ss) \<Longrightarrow>
+      A \<noteq> B \<Longrightarrow> disjoint (interval_of A) (interval_of B)"
     apply(induction ss arbitrary: rule: listwordinterval_compress.induct)
      apply(simp)
     apply(simp split: split_if_asm)
@@ -249,22 +299,22 @@ begin
   text\<open>END merging overlapping intervals\<close>
 
 
-
-
   text\<open>BEGIN merging adjacent intervals\<close>
-  private fun merge_adjacent :: "(('a::len) word \<times> ('a::len) word) \<Rightarrow> ('a word \<times> 'a word) list \<Rightarrow> ('a word \<times> 'a word) list" where
-     "merge_adjacent s [] = [s]" |
-     "merge_adjacent (s,e) ((s',e')#ss) = (
-        if s \<le>e \<and> s' \<le> e' \<and> word_next e = s'
-        then (s, e')#ss
-        else if s \<le>e \<and> s' \<le> e' \<and> word_next e' = s
-        then (s', e)#ss
-        else (s',e')#merge_adjacent (s,e) ss)"
+  private fun merge_adjacent
+    :: "(('a::len) word \<times> ('a::len) word) \<Rightarrow> ('a word \<times> 'a word) list \<Rightarrow> ('a word \<times> 'a word) list"
+  where
+    "merge_adjacent s [] = [s]" |
+    "merge_adjacent (s,e) ((s',e')#ss) = (
+       if s \<le>e \<and> s' \<le> e' \<and> word_next e = s'
+       then (s, e')#ss
+       else if s \<le>e \<and> s' \<le> e' \<and> word_next e' = s
+       then (s', e)#ss
+       else (s',e')#merge_adjacent (s,e) ss)"
 
   private lemma merge_adjacent_helper: 
   "interval_of A \<union> (\<Union>s \<in> set ss. interval_of s) = (\<Union>s \<in> set (merge_adjacent A ss). interval_of s)"
     apply(induction ss)
-     apply(simp)
+     apply(simp; fail)
     apply(rename_tac x xs)
     apply(cases A, rename_tac a b)
     apply(case_tac x)
@@ -277,7 +327,8 @@ begin
      using word_adjacent_union apply blast
     by blast
 
-  private lemma merge_adjacent_length: "\<exists>(s', e')\<in>set ss. s \<le> e \<and> s' \<le> e' \<and> (word_next e = s' \<or> word_next e' = s)
+  private lemma merge_adjacent_length:
+    "\<exists>(s', e')\<in>set ss. s \<le> e \<and> s' \<le> e' \<and> (word_next e = s' \<or> word_next e' = s)
      \<Longrightarrow> length (merge_adjacent (s,e) ss) = length ss"
     apply(induction ss)
      apply(simp)
@@ -286,7 +337,8 @@ begin
     apply(simp add: )
     by blast
 
-  private function listwordinterval_adjacent :: "(('a::len) word \<times> ('a::len) word) list \<Rightarrow> ('a word \<times> 'a word) list" where
+  private function listwordinterval_adjacent
+    :: "(('a::len) word \<times> ('a::len) word) list \<Rightarrow> ('a word \<times> 'a word) list" where
     "listwordinterval_adjacent [] = []" |
     "listwordinterval_adjacent ((s,e)#ss) = (
             if \<forall>(s',e') \<in> set ss. \<not> (s \<le>e \<and> s' \<le> e' \<and> (word_next e = s' \<or> word_next e' = s))
@@ -301,40 +353,57 @@ begin
   apply(simp)
   using merge_adjacent_length by fastforce
 
-  private lemma listwordinterval_adjacent: "(\<Union>s \<in> set (listwordinterval_adjacent ss). interval_of s) = (\<Union>s \<in> set ss. interval_of s)"
+  private lemma listwordinterval_adjacent:
+    "(\<Union>s \<in> set (listwordinterval_adjacent ss). interval_of s) = (\<Union>s \<in> set ss. interval_of s)"
     apply(induction ss rule: listwordinterval_adjacent.induct)
      apply(simp)
     apply(simp add: merge_adjacent_helper)
     done
 
-  value[code] "listwordinterval_adjacent [(1::16 word, 3), (5, 10), (10,10), (4,4)]"
+  lemma "listwordinterval_adjacent [(1::16 word, 3), (5, 10), (10,10), (4,4)] = [(10, 10), (1, 10)]"
+    by eval
   text\<open>END merging adjacent intervals\<close>
 
 
   definition wordinterval_compress :: "('a::len) wordinterval \<Rightarrow> 'a wordinterval" where
-    "wordinterval_compress r \<equiv> l2wi (remdups (listwordinterval_adjacent (listwordinterval_compress (wi2l (wordinterval_optimize_empty r)))))"
+    "wordinterval_compress r \<equiv>
+      l2wi (remdups (listwordinterval_adjacent (listwordinterval_compress
+        (wi2l (wordinterval_optimize_empty r)))))"
 
-  lemma wordinterval_compress: "wordinterval_to_set (wordinterval_compress r) = wordinterval_to_set r"
+  text\<open>Correctness: Compression preserves semantics\<close>
+  lemma wordinterval_compress:
+    "wordinterval_to_set (wordinterval_compress r) = wordinterval_to_set r"
     unfolding wordinterval_compress_def
     proof -
-      have interval_of': "\<And>s. interval_of s = (case s of (s,e) \<Rightarrow> {s .. e})" apply(case_tac s) using interval_of.simps by simp
+      have interval_of': "\<And>s. interval_of s = (case s of (s,e) \<Rightarrow> {s .. e})" apply(case_tac s)
+        using interval_of.simps by simp
 
-      have "wordinterval_to_set (l2wi (remdups (listwordinterval_adjacent (listwordinterval_compress (wi2l (wordinterval_optimize_empty r)))))) =
-            (\<Union>x\<in>set (listwordinterval_adjacent (listwordinterval_compress (wi2l (wordinterval_optimize_empty r)))). interval_of x)"
+      have "wordinterval_to_set (l2wi (remdups (listwordinterval_adjacent
+              (listwordinterval_compress (wi2l (wordinterval_optimize_empty r)))))) =
+            (\<Union>x\<in>set (listwordinterval_adjacent (listwordinterval_compress
+                (wi2l (wordinterval_optimize_empty r)))). interval_of x)"
       using l2wi l2wi_remdups interval_of.simps[symmetric] by blast
       also have "\<dots> =  (\<Union>s\<in>set (wi2l (wordinterval_optimize_empty r)). interval_of s)"
         by(simp add: listwordinterval_compress listwordinterval_adjacent)
-      also have "\<dots> = (\<Union>(i, j)\<in>set (wi2l (wordinterval_optimize_empty r)). {i..j})" by(simp add: interval_of')
+      also have "\<dots> = (\<Union>(i, j)\<in>set (wi2l (wordinterval_optimize_empty r)). {i..j})"
+        by(simp add: interval_of')
       also have "\<dots> = wordinterval_to_set r" by(simp add: wi2l)
       finally show "wordinterval_to_set
-        (l2wi (remdups (listwordinterval_adjacent (listwordinterval_compress (wi2l (wordinterval_optimize_empty r))))))
+        (l2wi (remdups (listwordinterval_adjacent (listwordinterval_compress
+            (wi2l (wordinterval_optimize_empty r))))))
           = wordinterval_to_set r" .
   qed
 
 end
 
-lemma "wordinterval_compress (RangeUnion (RangeUnion (WordInterval (1::32 word) 5) (WordInterval 8 10)) (WordInterval 3 7)) = WordInterval 1 0xA" by eval
+text\<open>Example\<close>
+lemma "(wi2l \<circ> (wordinterval_compress :: 32 wordinterval \<Rightarrow> 32 wordinterval) \<circ> l2wi)
+          [(70, 80001), (0,0), (150, 8000), (1,3), (42,41), (3,7), (56, 200), (8,10)] =
+          [(56, 80001), (0, 10)]" by eval
 
+lemma "wordinterval_compress (RangeUnion (RangeUnion (WordInterval (1::32 word) 5)
+                                                        (WordInterval 8 10)) (WordInterval 3 7)) =
+       WordInterval 1 10" by eval
 
 
 
@@ -344,13 +413,15 @@ subsection\<open>Further operations\<close>
   definition wordinterval_Union :: "('a::len) wordinterval list \<Rightarrow> 'a wordinterval" where
     "wordinterval_Union ws = wordinterval_compress (foldr wordinterval_union ws Empty_WordInterval)"
   
-  lemma wordinterval_Union: "wordinterval_to_set (wordinterval_Union ws) = (\<Union> w \<in> (set ws). wordinterval_to_set w)"
+  lemma wordinterval_Union:
+    "wordinterval_to_set (wordinterval_Union ws) = (\<Union> w \<in> (set ws). wordinterval_to_set w)"
     by(induction ws) (simp_all add: wordinterval_compress wordinterval_Union_def)
    
 
 context
 begin
-  private fun wordinterval_setminus' :: "'a::len wordinterval \<Rightarrow> 'a wordinterval \<Rightarrow> 'a wordinterval" where
+  private fun wordinterval_setminus'
+    :: "'a::len wordinterval \<Rightarrow> 'a wordinterval \<Rightarrow> 'a wordinterval" where
     "wordinterval_setminus' (WordInterval s e) (WordInterval ms me) = (
       if s > e \<or> ms > me then WordInterval s e else
       if me \<ge> e
@@ -360,12 +431,16 @@ begin
         then
           WordInterval (max s (word_next me)) (if me = max_word then 0 else e)
         else
-          RangeUnion (WordInterval (if ms = 0 then 1 else s) (word_prev ms)) (WordInterval (word_next me) (if me = max_word then 0 else e))
+          RangeUnion (WordInterval (if ms = 0 then 1 else s) (word_prev ms))
+                     (WordInterval (word_next me) (if me = max_word then 0 else e))
         )" |
-     "wordinterval_setminus' (RangeUnion r1 r2) t = RangeUnion (wordinterval_setminus' r1 t) (wordinterval_setminus' r2 t)"|
-     "wordinterval_setminus' t (RangeUnion r1 r2) = wordinterval_setminus' (wordinterval_setminus' t r1) r2"
+     "wordinterval_setminus' (RangeUnion r1 r2) t =
+        RangeUnion (wordinterval_setminus' r1 t) (wordinterval_setminus' r2 t)"|
+     "wordinterval_setminus' t (RangeUnion r1 r2) =
+        wordinterval_setminus' (wordinterval_setminus' t r1) r2"
 
-  private lemma wordinterval_setminus'_rr_set_eq: "wordinterval_to_set(wordinterval_setminus' (WordInterval s e) (WordInterval ms me)) = 
+  private lemma wordinterval_setminus'_rr_set_eq:
+    "wordinterval_to_set(wordinterval_setminus' (WordInterval s e) (WordInterval ms me)) = 
     wordinterval_to_set (WordInterval s e) - wordinterval_to_set (WordInterval ms me)"
      apply(simp only: wordinterval_setminus'.simps)
      apply(case_tac "e < s") 
@@ -403,17 +478,20 @@ begin
      apply(uint_arith)
    done
 
-  private lemma wordinterval_setminus'_set_eq: "wordinterval_to_set (wordinterval_setminus' r1 r2) = 
-    wordinterval_to_set r1 - wordinterval_to_set r2"
+  private lemma wordinterval_setminus'_set_eq:
+    "wordinterval_to_set (wordinterval_setminus' r1 r2) =
+      wordinterval_to_set r1 - wordinterval_to_set r2"
     apply(induction rule: wordinterval_setminus'.induct)
       using wordinterval_setminus'_rr_set_eq apply blast
      apply auto
     done
-  lemma wordinterval_setminus'_empty_struct: "wordinterval_empty r2 \<Longrightarrow> wordinterval_setminus' r1 r2 = r1"
+  lemma wordinterval_setminus'_empty_struct:
+    "wordinterval_empty r2 \<Longrightarrow> wordinterval_setminus' r1 r2 = r1"
     by(induction r1 r2 rule: wordinterval_setminus'.induct) auto
 
 
-  definition wordinterval_setminus :: "'a::len wordinterval \<Rightarrow> 'a::len wordinterval \<Rightarrow> 'a::len wordinterval" where
+  definition wordinterval_setminus
+    :: "'a::len wordinterval \<Rightarrow> 'a::len wordinterval \<Rightarrow> 'a::len wordinterval" where
     "wordinterval_setminus r1 r2 = wordinterval_compress (wordinterval_setminus' r1 r2)"
 
   lemma wordinterval_setminus_set_eq[simp]: "wordinterval_to_set (wordinterval_setminus r1 r2) = 
@@ -421,16 +499,19 @@ begin
     by(simp add: wordinterval_setminus_def wordinterval_compress wordinterval_setminus'_set_eq)
 end
 
-definition wordinterval_UNIV :: "'a::len wordinterval"where "wordinterval_UNIV \<equiv> WordInterval 0 max_word"
+definition wordinterval_UNIV :: "'a::len wordinterval" where
+  "wordinterval_UNIV \<equiv> WordInterval 0 max_word"
 lemma wordinterval_UNIV_set_eq[simp]: "wordinterval_to_set wordinterval_UNIV = UNIV"
   unfolding wordinterval_UNIV_def
   using max_word_max by fastforce
   
 fun wordinterval_invert :: "'a::len wordinterval \<Rightarrow> 'a::len wordinterval" where
   "wordinterval_invert r = wordinterval_setminus wordinterval_UNIV r"
-lemma wordinterval_invert_set_eq[simp]: "wordinterval_to_set (wordinterval_invert r) = UNIV - wordinterval_to_set r" by(auto)
+lemma wordinterval_invert_set_eq[simp]:
+  "wordinterval_to_set (wordinterval_invert r) = UNIV - wordinterval_to_set r" by(auto)
 
-lemma wordinterval_invert_UNIV_empty: "wordinterval_empty (wordinterval_invert wordinterval_UNIV)" by simp
+lemma wordinterval_invert_UNIV_empty:
+  "wordinterval_empty (wordinterval_invert wordinterval_UNIV)" by simp
 
 
 text\<open>@{text "\<inter>"}\<close>
@@ -438,7 +519,8 @@ context
 begin
   private lemma "{(s::nat) .. e} \<inter> {s' .. e'} = {} \<longleftrightarrow> s > e' \<or> s' > e \<or> s > e \<or> s' > e'"
     by simp linarith
-  private fun wordinterval_intersection' :: "'a::len wordinterval \<Rightarrow> 'a::len wordinterval \<Rightarrow> 'a::len wordinterval" where
+  private fun wordinterval_intersection'
+    :: "'a::len wordinterval \<Rightarrow> 'a::len wordinterval \<Rightarrow> 'a::len wordinterval" where
     "wordinterval_intersection' (WordInterval s e) (WordInterval s' e') = (
         if s > e \<or> s' > e' \<or> s > e' \<or> s' > e \<or> s > e \<or> s' > e'
         then
@@ -446,35 +528,48 @@ begin
         else
           WordInterval (max s s') (min e e')
         )" |
-    "wordinterval_intersection' (RangeUnion r1 r2) t = RangeUnion (wordinterval_intersection' r1 t) (wordinterval_intersection' r2 t)"|
-    "wordinterval_intersection' t (RangeUnion r1 r2) = RangeUnion (wordinterval_intersection' t r1) (wordinterval_intersection' t r2)"
+    "wordinterval_intersection' (RangeUnion r1 r2) t =
+        RangeUnion (wordinterval_intersection' r1 t) (wordinterval_intersection' r2 t)"|
+    "wordinterval_intersection' t (RangeUnion r1 r2) =
+        RangeUnion (wordinterval_intersection' t r1) (wordinterval_intersection' t r2)"
 
   private lemma wordinterval_intersection'_set_eq: 
-    "wordinterval_to_set (wordinterval_intersection' r1 r2) = wordinterval_to_set r1 \<inter> wordinterval_to_set r2"
+    "wordinterval_to_set (wordinterval_intersection' r1 r2) =
+      wordinterval_to_set r1 \<inter> wordinterval_to_set r2"
     by(induction r1 r2 rule: wordinterval_intersection'.induct) (auto)
 
-  value[code] "wordinterval_intersection' (RangeUnion (RangeUnion (WordInterval (1::32 word) 3) (WordInterval 8 10)) (WordInterval 1 3)) (WordInterval 1 3)"
+  lemma "wordinterval_intersection'
+          (RangeUnion (RangeUnion (WordInterval (1::32 word) 3) (WordInterval 8 10))
+                      (WordInterval 1 3)) (WordInterval 1 3) =
+          RangeUnion (RangeUnion (WordInterval 1 3) (WordInterval 1 0)) (WordInterval 1 3)" by eval
 
-  definition wordinterval_intersection :: "'a::len wordinterval \<Rightarrow> 'a::len wordinterval \<Rightarrow> 'a::len wordinterval" where 
+  definition wordinterval_intersection
+    :: "'a::len wordinterval \<Rightarrow> 'a::len wordinterval \<Rightarrow> 'a::len wordinterval" where 
     "wordinterval_intersection r1 r2 \<equiv> wordinterval_compress (wordinterval_intersection' r1 r2)"
 
   lemma wordinterval_intersection_set_eq[simp]: 
-    "wordinterval_to_set (wordinterval_intersection r1 r2) = wordinterval_to_set r1 \<inter> wordinterval_to_set r2"
-    (*unfolding wordinterval_intersection_def wordinterval_optimize_same_set_eq by auto*)
-    by(simp add: wordinterval_intersection_def wordinterval_compress wordinterval_intersection'_set_eq)
+    "wordinterval_to_set (wordinterval_intersection r1 r2) =
+      wordinterval_to_set r1 \<inter> wordinterval_to_set r2"
+    by(simp add: wordinterval_intersection_def
+                 wordinterval_compress wordinterval_intersection'_set_eq)
 
-  value[code] "wordinterval_intersection (RangeUnion (RangeUnion (WordInterval (1::32 word) 3) (WordInterval 8 10)) (WordInterval 1 3)) (WordInterval 1 3)"
+  lemma "wordinterval_intersection
+          (RangeUnion (RangeUnion (WordInterval (1::32 word) 3) (WordInterval 8 10))
+                      (WordInterval 1 3)) (WordInterval 1 3) =
+          WordInterval 1 3" by eval
 end
 
 
 definition wordinterval_subset :: "'a::len wordinterval \<Rightarrow> 'a::len wordinterval \<Rightarrow> bool" where
   "wordinterval_subset r1 r2 \<equiv> wordinterval_empty (wordinterval_setminus r1 r2)"
-lemma wordinterval_subset_set_eq[simp]: "wordinterval_subset r1 r2 = (wordinterval_to_set r1 \<subseteq> wordinterval_to_set r2)"
+lemma wordinterval_subset_set_eq[simp]:
+  "wordinterval_subset r1 r2 = (wordinterval_to_set r1 \<subseteq> wordinterval_to_set r2)"
   unfolding wordinterval_subset_def by simp
 
 definition wordinterval_eq :: "'a::len wordinterval \<Rightarrow> 'a::len wordinterval \<Rightarrow> bool" where 
   "wordinterval_eq r1 r2 = (wordinterval_subset r1 r2 \<and> wordinterval_subset r2 r1)"
-lemma wordinterval_eq_set_eq: "wordinterval_eq r1 r2 \<longleftrightarrow> wordinterval_to_set r1 = wordinterval_to_set r2"
+lemma wordinterval_eq_set_eq:
+  "wordinterval_eq r1 r2 \<longleftrightarrow> wordinterval_to_set r1 = wordinterval_to_set r2"
   unfolding wordinterval_eq_def by auto
 
 thm iffD1[OF wordinterval_eq_set_eq]
@@ -485,9 +580,11 @@ lemma wordinterval_eq_comm: "wordinterval_eq r1 r2 \<longleftrightarrow> wordint
 lemma wordinterval_to_set_alt: "wordinterval_to_set r = {x. wordinterval_element x r}"
   unfolding wordinterval_element_set_eq by blast
 
-lemma wordinterval_un_empty: "wordinterval_empty r1 \<Longrightarrow> wordinterval_eq (wordinterval_union r1 r2) r2"
+lemma wordinterval_un_empty:
+  "wordinterval_empty r1 \<Longrightarrow> wordinterval_eq (wordinterval_union r1 r2) r2"
   by(subst wordinterval_eq_set_eq, simp)
-lemma wordinterval_un_emty_b: "wordinterval_empty r2 \<Longrightarrow> wordinterval_eq (wordinterval_union r1 r2) r1"
+lemma wordinterval_un_emty_b:
+  "wordinterval_empty r2 \<Longrightarrow> wordinterval_eq (wordinterval_union r1 r2) r1"
   by(subst wordinterval_eq_set_eq, simp)
 
 lemma wordinterval_Diff_triv: 
@@ -497,7 +594,7 @@ lemma wordinterval_Diff_triv:
 
 
 
-
+text\<open>A size of the datatype, does not correspond to the cardinality of the corresponding set\<close>
 fun wordinterval_size :: "('a::len) wordinterval \<Rightarrow> nat" where
   "wordinterval_size (RangeUnion a b) = wordinterval_size a + wordinterval_size b" |
   "wordinterval_size (WordInterval s e) = (if s \<le> e then 1 else 0)"
@@ -506,9 +603,7 @@ lemma wordinterval_size_length: "wordinterval_size r = length (wi2l r)"
   by(induction r) (auto)
 
 lemma Ex_wordinterval_nonempty: "\<exists>x::('a::len wordinterval). y \<in> wordinterval_to_set x"
-proof show "y \<in> wordinterval_to_set wordinterval_UNIV" by simp qed
-
-
+  proof show "y \<in> wordinterval_to_set wordinterval_UNIV" by simp qed
 
 lemma wordinterval_eq_reflp:
   "reflp wordinterval_eq"
@@ -528,9 +623,9 @@ lemma wordinterval_eq_equivp:
   by (auto intro: equivpI wordinterval_eq_reflp wordintervalt_eq_symp wordinterval_eq_transp)
 
 
- definition is_lowest_element :: "'a::ord \<Rightarrow> 'a set \<Rightarrow> bool" where
-  "is_lowest_element x S = (x \<in> S \<and> (\<forall>y\<in>S. y \<le> x \<longrightarrow> y = x))"
-
+text\<open>The smallest element in the interval\<close>
+  definition is_lowest_element :: "'a::ord \<Rightarrow> 'a set \<Rightarrow> bool" where
+    "is_lowest_element x S = (x \<in> S \<and> (\<forall>y\<in>S. y \<le> x \<longrightarrow> y = x))"
 
   lemma 
   	fixes x :: "'a :: complete_lattice"
@@ -550,14 +645,15 @@ lemma wordinterval_eq_equivp:
    using assms by(auto)
   by (metis Min.coboundedI assms(1) assms(2) dual_order.antisym is_lowest_element_def)
 
-    
+text\<open>Smallest element in the interval\<close>
   fun wordinterval_lowest_element :: "'a::len0 wordinterval \<Rightarrow> 'a word option" where
     "wordinterval_lowest_element (WordInterval s e) = (if s \<le> e then Some s else None)" | 
-    "wordinterval_lowest_element (RangeUnion A B) = (case (wordinterval_lowest_element A, wordinterval_lowest_element B) of
-      (Some a, Some b) \<Rightarrow> Some (if a < b then a else b) |
-      (None, Some b) \<Rightarrow> Some b |
-      (Some a, None) \<Rightarrow> Some a |
-      (None, None) \<Rightarrow> None)"
+    "wordinterval_lowest_element (RangeUnion A B) =
+      (case (wordinterval_lowest_element A, wordinterval_lowest_element B) of
+          (Some a, Some b) \<Rightarrow> Some (if a < b then a else b) |
+          (None, Some b) \<Rightarrow> Some b |
+          (Some a, None) \<Rightarrow> Some a |
+          (None, None) \<Rightarrow> None)"
 
   lemma wordinterval_lowest_none_empty: "wordinterval_lowest_element r = None \<longleftrightarrow> wordinterval_empty r"
     proof(induction r)
@@ -567,7 +663,8 @@ lemma wordinterval_eq_equivp:
     qed
     
 
-  lemma wordinterval_lowest_element_correct_A: "wordinterval_lowest_element r = Some x \<Longrightarrow> is_lowest_element x (wordinterval_to_set r)"
+  lemma wordinterval_lowest_element_correct_A:
+    "wordinterval_lowest_element r = Some x \<Longrightarrow> is_lowest_element x (wordinterval_to_set r)"
     unfolding is_lowest_element_def
     apply(induction r arbitrary: x rule: wordinterval_lowest_element.induct)
      apply(rename_tac rs re x, case_tac "rs \<le> re", auto)[1]
@@ -600,7 +697,9 @@ lemma wordinterval_eq_equivp:
           by(simp add: is_lowest_element_def)
       
          (*why \<And> A B?*)
-         have wordinterval_lowest_element_RangeUnion: "\<And>a b A B. wordinterval_lowest_element A = Some a \<Longrightarrow> wordinterval_lowest_element B = Some b \<Longrightarrow>
+         have wordinterval_lowest_element_RangeUnion:
+          "\<And>a b A B. wordinterval_lowest_element A = Some a \<Longrightarrow>
+                  wordinterval_lowest_element B = Some b \<Longrightarrow>
                   wordinterval_lowest_element (RangeUnion A B) = Some (min a b)"
            by(auto dest!: wordinterval_lowest_element_correct_A simp add: is_lowest_element_def min_def)
          
@@ -629,11 +728,6 @@ lemma wordinterval_eq_equivp:
 text\<open>Cardinality approximation for @{typ "('a::len) wordinterval"}s\<close>
 context
 begin
-  lemma card_enum_upto: fixes s::"('a::len) word" shows "card (set [s .e. e]) = Suc (unat e) - unat s"
-    apply(subst List.card_set)
-    apply(simp add: remdups_enum_upto)
-    done
-  
   lemma card_atLeastAtMost_word: fixes s::"('a::len) word" shows "card {s..e} = Suc (unat e) - (unat s)"
     apply(cases "s > e")
      apply(simp)
@@ -653,7 +747,8 @@ begin
     case WordInterval thus ?case by (simp add: card_atLeastAtMost_word)
     next
     case (RangeUnion r1 r2)
-      have "card (wordinterval_to_set r1 \<union> wordinterval_to_set r2) \<le> card (wordinterval_to_set r1) + card (wordinterval_to_set r2)"
+      have "card (wordinterval_to_set r1 \<union> wordinterval_to_set r2) \<le>
+              card (wordinterval_to_set r1) + card (wordinterval_to_set r2)"
         using Finite_Set.card_Un_le by blast
       with RangeUnion show ?case by(simp)
     qed
